src/classes/SMT_classes_instances.v
@@ -748,5 +748,3 @@ Section prod.
   |}.
 
 End prod.
-
-Hint Resolve unit_compdec bool_compdec Z_compdec Nat_compdec Positive_compdec BV_compdec FArray_compdec int63_compdec option_compdec list_compdec prod_compdec : typeclass_instances.
